---
date: "2024-01-08"
id: A1
modified: 2025-10-29 02:16:19 GMT-04:00
tags:
  - sfwr2c03
title: Time complexity and recurrence relations
---

## Problem 1

### 1.1

Consider the following function of $n$:

$$
\begin{aligned}
&n^2 \quad \sum_{i=0}^{n}5\cdot{i} \quad n^3\cdot \sqrt{\frac{1}{n^3}} \quad n^2 + 2^n \quad (\Pi_{i=1}^{9}i) \quad (\sum_{i=0}^{\log_2(n)}2^i) + 1 \quad 7^{\ln{(n)}} \\
&-\ln{(\frac{1}{n})} \quad \ln{(2^n)} \quad 10 \quad n\log_2{(n^7)} \quad \sqrt{n^4} \quad n^n \quad 5n \\
\end{aligned}
$$

Group the above functions that have identical growth rate and order these groups on increasing
growth. Hence:

- If you place functions $f_1(n)$ and $f_2(n)$ in the same group, then we must have $f_1(n) = \Theta{(f_2(n))}$;

- If you place function $f_1(n)$ in a group ordered before the group in which you place function $f_2(n)$,
  then we must have $f_1(n) = \mathcal{O}{(f_2(n))} \land f_1(n) \neq \Omega{(f_2(n))}$.

_Solution:_

Theorem 3.25 states the following:

$$
\lim_{n \to \infty} \frac{f(n)}{g(n)} \space \text{is defined and is} \space
\begin{cases}
  \infty & \space \text{then} \space f(n) = \Omega(g(n)); \\
  c \text{, with c > 0  a constant} & \space \text{then} \space f(n) = \Theta(g(n)); \\
  0 & \space \text{then} \space f(n) = \mathcal{O}(g(n));
\end{cases}
$$

The following are the rules of thumb to determine the order of growth of functions:

$$
\begin{align}
c \cdot f(n) &= \Theta(f(n)) \\
\log_{a}(n) &= \Theta(\log_{b}(n)) \\
\lim_{n \to \infty} \frac{n^c}{n^{c+d}} &= \lim_{n \to \infty} \frac{1}{n^d} = 0 \rightarrow n^c = \mathcal{O}(n^{c+d}) \\
\log_{2}(n)^c &= \mathcal{O}(n^d) \space \forall c > 0, d > 0 \\
n^c &= \mathcal{O}(d^{n}) \space \forall c > 0, d > 1 \\
d^{\frac{n}{u}} &= \mathcal{O}(c^{\frac{n}{v}}) \space \forall c \geq d \geq 1, u \geq v \geq 1 \\
\sum_{i=1}^{m}{c_{i} \cdot n^{d_i}} &= \mathcal{O}(n^{d_i}) \\
f(n) + g(n) &= \Theta(g(n)) \\
h(n) \cdot n(n) &= \mathcal{O}({h(n) \cdot g(n)})
\end{align}
$$

Let's start with analysing the functions that have the same growth rate:

- $n^2$: polynomial growth, $n^2 = \Theta(n^2)$ based on rule 3.

- $\sum_{i=0}^{n}5\cdot{i}$: polynomial growth, $\sum_{i=0}^{n}5\cdot{i} = 5 \cdot \frac{n(n+1)}{2} = \frac{5}{2}n^2 + \frac{5}{2}n$, which is $\Theta(n^2)$ based on rule $7$.

- $n^3 \cdot \sqrt{\frac{1}{n^3}}$: polynomial growth, $= n^3 \cdot \frac{1}{n^{\frac{3}{2}}} \rightarrow \Theta(n^{\frac{3}{2}})$ based on rule $9, 3$

- $n^2 + 2^n$: exponential growth, $=\Theta(2^n)$ based on rule $7$

- $(\Pi_{i=1}^{9}i)$: constant, $=1 \cdot 2 \dots 9$ based on rule 9

- $\sum_{i=0}^{\log_2{(n)}}{2^i} + 1$: linear, since the term is a geometrics series, such that $\sum_{i=0}^{\log_2{(n)}}{2^i} + 1 = \frac{1 \cdot (2^{\log_2(n)+1}-1)}{2-1} + 1 = 2 \cdot 2^{\log_2(n)} = 2n$. Therefore based on rule $1$ we have $\Theta(n)$

- $7^{\ln(n)}$: polynomial, since $7^{\ln(n)} = n^{\ln(7)}$. Apply rule $3$ we have $7^{\ln(n)} = \Theta(n^{\ln 7}) \rightarrow \mathcal{O}(n^2)$

- $-\ln(\frac{1}{n})$: logarithmic, since $-\ln (\frac{1}{n}) = \ln(n)$. Apply rule $1$ yield $\Theta{(\ln{n})}$.

- $\ln (2^n)$: linear, since $\ln(2^n) = n \cdot \ln_{2}$ and rule $1$ yield $\Theta{(n)}$

- $10$: constant

- $n\log_2(n^7)$: polynomial, since $n\log_{2}(n^7) = n \cdot 7\log_{2}{(n)} = 7n\log_{2}(n)$. Based on rule $9$ and $1$ yield $\mathcal{O}(n^2)$

- $\sqrt{n^4}$: polynomial growth, $=n^2$ based on rule 3.

- $n^n$: super-exponential.

- $5n$: linear based on rule 1, gives $\Theta(n)$

Thus the order from increasing rate:

- $10 \quad (\Pi_{i=1}^{9}i)$ (_constant_)

- $-\ln(\frac{1}{n})$ (_logarithmic_)

- $\ln (2^n) \quad 5n \quad \sum_{i=0}^{\log_2{(n)}}{2^i} + 1$ (_linear_)

- $n^2 \quad \sum_{i=0}^{n}5\cdot{i} \quad n^3 \cdot \sqrt{\frac{1}{n^3}} \quad \sqrt{n^4} \quad n\log_2(n^7) \quad 7^{\ln(n)}$ (_polynomial_)

- $n^2 + 2^n$ (_exponential_)

- $n^n$ (_super-exponential_)

### 1.2

Consider the following recurrence

$$
T(n) = \begin{cases}
    7 & \text{if } n \leq 1;\\
    3T(n-2) & \text{if } n > 1.
\end{cases}
$$

Use induction to prove that $T(n) = f(n)$ with $f(n) = 7 \cdot 3^{[\frac{n}{2}]}$

_Solution:_

#### base case:

Given $T(n) = f(n) = 7 \cdot 3^{[\frac{n}{2}]}$ apply for $n=0$ and $n=1$:

- $n = 1 \rightarrow T(n) = 7 \cdot 3^{[\frac{1}{2}]} = 7 \cdot 3^0 = 7$
- $n = 0 \rightarrow T(n) = 7 \cdot 3^{[\frac{0}{2}]} = 7 \cdot 3^0 = 7$

Thus the base case holds.

#### induction hypothesis:

Assume $T(n) = f(n)$ holds for $n > 1$. We will proves that $f(n+2) = T(n+2)$ also holds.

$$
\begin{align}
f(n) &= T(n) \\
T(n) = f(n) &= 3T(n-2) = 3f(n-2) = 3 \cdot 7 \cdot 3^{[\frac{n-2}{2}]} \\
T(n+2) &= 3T(n)
\end{align}
$$

Therefore:

$$
\begin{align}
T(n+2) &= 3 \cdot 3 \cdot 7 \cdot 3^{[\frac{n-2}{2}]} = 7 \cdot 3^{[\frac{n-2}{2} + 2]} \\
T(n+2) &= 7 \cdot 3^{[\frac{n+2}{2}]} = f(n+2)
\end{align}
$$

Therefore the induction hypothesis holds.

#### conclusion:

> $T(n) = f(n) = 7 \cdot 3^{[\frac{n}{2}]}$ is true for all $n \geq 0$.

---

## Problem 2

Consider the following `Count` algorithm

```prolog
Algorithm Count(L, v):
Pre: L is an array, v is a value
i, c := 0, 0
while i neq |L| do
  if L[i] = v then
    c := c + 1
 end if
 i := i + 1
end while
return c.
Post: return the number of copies of v in L
```

### 2.1

Provide an invariant for the while loop at Line 2

_Solution_:

$$
0 \leq i \leq |L|, c = \sum_{j=0}^{i-1} \lbrack L \lbrack j \rbrack = v \rbrack
$$

### 2.2

Provide a bound function for the while loop at Line 2

_Solution_:

$$
f(i) = |L| - i
$$

### 2.3

Prove that `Count` algorithm is correct.

_Solution:_

Line 1: `i, c := 0, 0`

- $L \lbrack 0, i)$ with $i=0$ is $L \lbrack 0, 0)$

- $L \lbrack 0,0)$ is empty, hence $c = \sum_{j=0}^{i-1} \lbrack L \lbrack j \rbrack = v \rbrack  = 0$

- bound function $f(i) = |L| - i$ starts at $|L|, |L| \geq 0$

Line 2: `while i neq |L| do`

- bound function $f(i)$ stops at $0$

- invariant still holds, with $i \neq |L|$

Now prove invariant holds again til reach the end of the `m-th` loop:

Line 3-5: `if L[i] = v then` case:

- $L \lbrack i \rbrack = v$ hence $v \in L\lbrack 0,i \rbrack$
- invariant still holds, with $i \neq |L|$ and $L\lbrack v \rbrack = v$
- $i_{\text{new}} = i + 1$ hence $0 < i_{\text{new}} \leq |L|$ implies $ 0 \leq i*{\text{new}} \leq |L|$ and $f(i*{\text{new}}) = f(i) - 1$
- $c_{\text{new}} = c + 1 = \sum_{j=0}^{i-1} \lbrack L \lbrack j \rbrack = v \rbrack + 1 = \sum_{j=0}^{i_{\text{new}}} \lbrack L \lbrack j \rbrack = v \rbrack$

- $f(i)$ strictly decreases after each iteration, $i_{\text{new}} := i + 1$

Therefore the invariant still holds within the if statement.

L7: `end while`

- $i = |L|$ hence $f(i) = 0$, the loop stops
- $c = \sum_{j=0}^{i-1} \lbrack L \lbrack j \rbrack = v \rbrack = \sum_{j=0}^{|L|-1} \lbrack L \lbrack j \rbrack = v \rbrack$

Therefore the invariant still holds at the end of the loop.

### 2.4

What is the runtime and memory complexity of `Count` algorithm?

_Solution:_

- L1 implies 2 instructions
- L2 implies 2 instructions $|L| + 1$ times,
- L3-5 (if loop) implies 4 instructions $|L|$ times
- L6 implies 2 instructions $|L|$ times

Therefore number of work is $5 + 8N$, thus runtime complexity would be $\Theta(5+8N)$.

Memory complexity is $\Theta(1)$, since only 2 variables are used.

### 2.5

Provide an algorithm `FastCount(L, v)` operates on ordered lists `L` and computes the same results as `Count(L, v)` but with a $\mathcal{O}(\log_2(|L|))$

_Solution:_

```prolog
Algorithm FastCount(L, v):
Pre: L is an ordered array, v is a value
function binarySearchFirst(L, v)
  low, high := 0, |L| - 1
  results := -1
  while low <= high do
    mid := (low + high) / 2
    if L[mid] < v then
      low := mid + 1
    else if L[mid] > v then
      high := mid - 1
    else
      results := mid
      high := mid - 1
  end while
  return results
end function

function binarySearchLast(L, v)
  low, high := 0, |L| - 1
  results := -1
  while low <= high do
    mid := (low + high) / 2
    if L[mid] < v then
      low := mid + 1
    else if L[mid] > v then
      high := mid - 1
    else
      results := mid
      low := mid + 1
  end while
  return result
end function

firstIndex := binarySearchFirst(L, v)
if firstIndex = -1 then
  return 0
end if
lastIndex := binarySearchLast(L, v)
return lastIndex - firstIndex + 1
Post: return the number of copies of v in L
```
